utp_rel_laws.thy
@@ -7,21 +7,27 @@ theory utp_rel_laws
     utp_liberate
 begin
 
+lemma rcond_true [simp]: "P \<^bold>\<lhd> true \<^bold>\<rhd> Q = P"
+  by (simp add: rel_eq_iff rel_rcond)
+
+lemma rcond_false [simp]: "(P \<^bold>\<lhd> false \<^bold>\<rhd> Q) = Q"
+  by (simp add: rel_eq_iff rel_rcond)
+
 lemma comp_cond_left_distr:
-  "(P \<^bold>\<lhd> b \<^bold>\<rhd> Q) ;; R = (P ;; R) \<^bold>\<lhd> b \<^bold>\<rhd> (Q ;; R) "
+  "(P \<^bold>\<lhd> b \<^bold>\<rhd> Q) \<Zcomp> R = (P \<Zcomp> R) \<^bold>\<lhd> b \<^bold>\<rhd> (Q \<Zcomp> R) "
   by (rel_auto)
 
 lemma cond_seq_left_distr:
-  "out\<alpha> \<sharp> b \<Longrightarrow> ((P \<lhd> b \<rhd> Q) ;; R) = ((P ;; R) \<lhd> b \<rhd> (Q ;; R))"
+  "out\<alpha> \<sharp> b \<Longrightarrow> ((P \<lhd> b \<rhd> Q) \<Zcomp> R) = ((P \<Zcomp> R) \<lhd> b \<rhd> (Q \<Zcomp> R))"
   by (rel_auto, blast)
 
 lemma cond_seq_right_distr:
-  "in\<alpha> \<sharp> b \<Longrightarrow> (P ;; (Q \<lhd> b \<rhd> R)) = ((P ;; Q) \<lhd> b \<rhd> (P ;; R))"
+  "in\<alpha> \<sharp> b \<Longrightarrow> (P \<Zcomp> (Q \<lhd> b \<rhd> R)) = ((P \<Zcomp> Q) \<lhd> b \<rhd> (P \<Zcomp> R))"
   by (rel_auto, blast)
 
 text \<open> Alternative expression of conditional using assumptions and choice \<close>
 
-lemma rcond_rassume_expand: "P \<^bold>\<lhd> b \<^bold>\<rhd> Q = (\<questiondown>b? ;; P) \<union> (\<questiondown>(\<not> b)? ;; Q)"
+lemma rcond_rassume_expand: "P \<^bold>\<lhd> b \<^bold>\<rhd> Q = (\<questiondown>b? \<Zcomp> P) \<union> (\<questiondown>(\<not> b)? \<Zcomp> Q)"
   by rel_auto
 
 lemma rcond_mono:  "\<lbrakk> P\<^sub>1 \<sqsubseteq> P\<^sub>2; Q\<^sub>1 \<sqsubseteq> Q\<^sub>2 \<rbrakk> \<Longrightarrow> (P\<^sub>1 \<^bold>\<lhd> b \<^bold>\<rhd> Q\<^sub>1) \<sqsubseteq> (P\<^sub>2 \<^bold>\<lhd> b \<^bold>\<rhd> Q\<^sub>2)"
@@ -30,213 +36,213 @@ lemma rcond_mono:  "\<lbrakk> P\<^sub>1 \<sqsubseteq> P\<^sub>2; Q\<^sub>1 \<sqs
 subsection \<open> Precondition and Postcondition Laws \<close>
   
 theorem precond_equiv:
-  "P = (P ;; true) \<longleftrightarrow> (out\<alpha> \<sharp> P)"
+  "P = (P \<Zcomp> true) \<longleftrightarrow> (out\<alpha> \<sharp> P)"
   by (rel_auto)
 
 theorem postcond_equiv:
-  "P = (true ;; P) \<longleftrightarrow> (in\<alpha> \<sharp> P)"
+  "P = (true \<Zcomp> P) \<longleftrightarrow> (in\<alpha> \<sharp> P)"
   by (rel_auto)
 
 theorem precond_left_zero:
   assumes "out\<alpha> \<sharp> p" "p \<noteq> false"
-  shows "(true ;; p) = true"
+  shows "(true \<Zcomp> p) = true"
   using assms by (rel_auto)
 
 (*theorem feasibile_iff_true_right_zero:
-  "P ;; true = true \<longleftrightarrow> (\<exists> out\<alpha> \<bullet> P)\<^sub>u"
+  "P \<Zcomp> true = true \<longleftrightarrow> (\<exists> out\<alpha> \<bullet> P)\<^sub>u"
   oops*)
     
 subsection \<open> Sequential Composition Laws \<close>
     
-lemma seqr_assoc: "(P ;; Q) ;; R = P ;; (Q ;; R)"
+lemma seqr_assoc: "(P \<Zcomp> Q) \<Zcomp> R = P \<Zcomp> (Q \<Zcomp> R)"
   by (rel_auto)
 
 lemma seqr_left_zero [simp]:
-  "false ;; P = false"
+  "false \<Zcomp> P = false"
   by pred_auto
 
 lemma seqr_right_zero [simp]:
-  "P ;; false = false"
+  "P \<Zcomp> false = false"
   by pred_auto
 
 lemma seqr_mono:
-  "\<lbrakk> P\<^sub>1 \<sqsubseteq> P\<^sub>2; Q\<^sub>1 \<sqsubseteq> Q\<^sub>2 \<rbrakk> \<Longrightarrow> (P\<^sub>1 ;; Q\<^sub>1) \<sqsubseteq> (P\<^sub>2 ;; Q\<^sub>2)"
+  "\<lbrakk> P\<^sub>1 \<sqsubseteq> P\<^sub>2; Q\<^sub>1 \<sqsubseteq> Q\<^sub>2 \<rbrakk> \<Longrightarrow> (P\<^sub>1 \<Zcomp> Q\<^sub>1) \<sqsubseteq> (P\<^sub>2 \<Zcomp> Q\<^sub>2)"
   by (rel_auto)
     
 lemma seqr_monotonic:
-  "\<lbrakk> mono P; mono Q \<rbrakk> \<Longrightarrow> mono (\<lambda> X. P X ;; Q X)"
+  "\<lbrakk> mono P; mono Q \<rbrakk> \<Longrightarrow> mono (\<lambda> X. P X \<Zcomp> Q X)"
   by (simp add: mono_def relcomp_mono)
 
 (*
 lemma Monotonic_seqr_tail [closure]:
   assumes "Monotonic F"
-  shows "Monotonic (\<lambda> X. P ;; F(X))"
+  shows "Monotonic (\<lambda> X. P \<Zcomp> F(X))"
   by (simp add: assms monoD monoI seqr_mono) *)
 
-lemma seqr_liberate_left: "vwb_lens x \<Longrightarrow> (((P :: 'a \<leftrightarrow> 'b) \\ $x\<^sup><) ;; Q) = ((P ;; Q) \\ $x\<^sup><)"
+lemma seqr_liberate_left: "vwb_lens x \<Longrightarrow> (((P :: 'a \<leftrightarrow> 'b) \\ $x\<^sup><) \<Zcomp> Q) = ((P \<Zcomp> Q) \\ $x\<^sup><)"
   by (rel_auto add: liberate_pred_def)
 
-lemma seqr_liberate_right: "vwb_lens x \<Longrightarrow> P ;; Q \\ $x\<^sup>> = (P ;; Q) \\ $x\<^sup>>"
+lemma seqr_liberate_right: "vwb_lens x \<Longrightarrow> P \<Zcomp> Q \\ $x\<^sup>> = (P \<Zcomp> Q) \\ $x\<^sup>>"
   by (rel_auto add: liberate_pred_def)
 
 lemma seqr_or_distl:
-  "((P \<or> Q) ;; R) = ((P ;; R) \<or> (Q ;; R))"
+  "((P \<or> Q) \<Zcomp> R) = ((P \<Zcomp> R) \<or> (Q \<Zcomp> R))"
   by (rel_auto)
 
 lemma seqr_or_distr:
-  "(P ;; (Q \<or> R)) = ((P ;; Q) \<or> (P ;; R))"
+  "(P \<Zcomp> (Q \<or> R)) = ((P \<Zcomp> Q) \<or> (P \<Zcomp> R))"
   by (rel_auto)
 
 (*
 lemma seqr_and_distr_ufunc:
-  "ufunctional P \<Longrightarrow> (P ;; (Q \<and> R)) = ((P ;; Q) \<and> (P ;; R))"
+  "ufunctional P \<Longrightarrow> (P \<Zcomp> (Q \<and> R)) = ((P \<Zcomp> Q) \<and> (P \<Zcomp> R))"
   by (rel_auto)
 
 lemma seqr_and_distl_uinj:
-  "uinj R \<Longrightarrow> ((P \<and> Q) ;; R) = ((P ;; R) \<and> (Q ;; R))"
+  "uinj R \<Longrightarrow> ((P \<and> Q) \<Zcomp> R) = ((P \<Zcomp> R) \<and> (Q \<Zcomp> R))"
   by (rel_auto)
 
 lemma seqr_unfold:
-  "(P ;; Q) = (\<^bold>\<exists> v \<bullet> P\<lbrakk>\<guillemotleft>v\<guillemotright>/$\<^bold>v\<acute>\<rbrakk> \<and> Q\<lbrakk>\<guillemotleft>v\<guillemotright>/$\<^bold>v\<rbrakk>)"
+  "(P \<Zcomp> Q) = (\<^bold>\<exists> v \<bullet> P\<lbrakk>\<guillemotleft>v\<guillemotright>/$\<^bold>v\<acute>\<rbrakk> \<and> Q\<lbrakk>\<guillemotleft>v\<guillemotright>/$\<^bold>v\<rbrakk>)"
   by (rel_auto)
 
 lemma seqr_unfold_heterogeneous:
-  "(P ;; Q) = (pre(P\<lbrakk>\<guillemotleft>v\<guillemotright>//$v\<^sup>>\<rbrakk>))\<^sup>< \\ v\<^sup>< \<and> (post(Q\<lbrakk>\<guillemotleft>v\<guillemotright>/$v\<rbrakk>))\<^sup>>)"
+  "(P \<Zcomp> Q) = (pre(P\<lbrakk>\<guillemotleft>v\<guillemotright>//$v\<^sup>>\<rbrakk>))\<^sup>< \\ v\<^sup>< \<and> (post(Q\<lbrakk>\<guillemotleft>v\<guillemotright>/$v\<rbrakk>))\<^sup>>)"
   by (rel_auto)
 
 lemma seqr_middle:
   assumes "vwb_lens x"
-  shows "(P ;; Q) = (\<^bold>\<exists> v \<bullet> P\<lbrakk>\<guillemotleft>v\<guillemotright>/$x\<acute>\<rbrakk> ;; Q\<lbrakk>\<guillemotleft>v\<guillemotright>/$x\<rbrakk>)"
+  shows "(P \<Zcomp> Q) = (\<^bold>\<exists> v \<bullet> P\<lbrakk>\<guillemotleft>v\<guillemotright>/$x\<acute>\<rbrakk> \<Zcomp> Q\<lbrakk>\<guillemotleft>v\<guillemotright>/$x\<rbrakk>)"
   using assms
   by (rel_auto', metis vwb_lens_wb wb_lens.source_stability)
 *)
 
 lemma seqr_left_one_point:
   assumes "vwb_lens x"
-  shows "((P \<and> ($x\<^sup>> = \<guillemotleft>v\<guillemotright>)\<^sub>u) ;; Q) = (P\<lbrakk>\<guillemotleft>v\<guillemotright>/x\<^sup>>\<rbrakk> ;; Q\<lbrakk>\<guillemotleft>v\<guillemotright>/x\<^sup><\<rbrakk>)"
+  shows "((P \<and> ($x\<^sup>> = \<guillemotleft>v\<guillemotright>)\<^sub>u) \<Zcomp> Q) = (P\<lbrakk>\<guillemotleft>v\<guillemotright>/x\<^sup>>\<rbrakk> \<Zcomp> Q\<lbrakk>\<guillemotleft>v\<guillemotright>/x\<^sup><\<rbrakk>)"
   using assms
   by (rel_auto, metis vwb_lens_wb wb_lens.get_put)
 
 lemma seqr_right_one_point:
   assumes "vwb_lens x"
-  shows "(P ;; (($x\<^sup>< = \<guillemotleft>v\<guillemotright>)\<^sub>u \<and> Q)) = (P\<lbrakk>\<guillemotleft>v\<guillemotright>/x\<^sup>>\<rbrakk> ;; Q\<lbrakk>\<guillemotleft>v\<guillemotright>/x\<^sup><\<rbrakk>)"
+  shows "(P \<Zcomp> (($x\<^sup>< = \<guillemotleft>v\<guillemotright>)\<^sub>u \<and> Q)) = (P\<lbrakk>\<guillemotleft>v\<guillemotright>/x\<^sup>>\<rbrakk> \<Zcomp> Q\<lbrakk>\<guillemotleft>v\<guillemotright>/x\<^sup><\<rbrakk>)"
   using assms
   by (rel_auto, metis vwb_lens_wb wb_lens.get_put)
 
 lemma seqr_left_one_point_true:
   assumes "vwb_lens x"
-  shows "((P \<and> ($x\<^sup>>)\<^sub>u) ;; Q) = (P\<lbrakk>true/x\<^sup>>\<rbrakk> ;; Q\<lbrakk>true/x\<^sup><\<rbrakk>)"
+  shows "((P \<and> ($x\<^sup>>)\<^sub>u) \<Zcomp> Q) = (P\<lbrakk>true/x\<^sup>>\<rbrakk> \<Zcomp> Q\<lbrakk>true/x\<^sup><\<rbrakk>)"
   using assms
   by (rel_auto, metis (full_types) vwb_lens_wb wb_lens.get_put)
 
 lemma seqr_left_one_point_false:
   assumes "vwb_lens x"
-  shows "((P \<and> \<not>($x\<^sup>>)\<^sub>u) ;; Q) = (P\<lbrakk>false/x\<^sup>>\<rbrakk> ;; Q\<lbrakk>false/x\<^sup><\<rbrakk>)"
+  shows "((P \<and> \<not>($x\<^sup>>)\<^sub>u) \<Zcomp> Q) = (P\<lbrakk>false/x\<^sup>>\<rbrakk> \<Zcomp> Q\<lbrakk>false/x\<^sup><\<rbrakk>)"
   using assms by (rel_auto, metis (full_types) vwb_lens_wb wb_lens.get_put)
 
 lemma seqr_right_one_point_true:
   assumes "vwb_lens x"
-  shows "(P ;; (($x\<^sup><)\<^sub>u \<and> Q)) = (P\<lbrakk>true/x\<^sup>>\<rbrakk> ;; Q\<lbrakk>true/x\<^sup><\<rbrakk>)"
+  shows "(P \<Zcomp> (($x\<^sup><)\<^sub>u \<and> Q)) = (P\<lbrakk>true/x\<^sup>>\<rbrakk> \<Zcomp> Q\<lbrakk>true/x\<^sup><\<rbrakk>)"
   using assms by (rel_auto, metis (full_types) vwb_lens_wb wb_lens.get_put)
 
 lemma seqr_right_one_point_false:
   assumes "vwb_lens x"
-  shows "(P ;; (\<not>($x\<^sup><)\<^sub>u \<and> Q)) = (P\<lbrakk>false/x\<^sup>>\<rbrakk> ;; Q\<lbrakk>false/x\<^sup><\<rbrakk>)"
+  shows "(P \<Zcomp> (\<not>($x\<^sup><)\<^sub>u \<and> Q)) = (P\<lbrakk>false/x\<^sup>>\<rbrakk> \<Zcomp> Q\<lbrakk>false/x\<^sup><\<rbrakk>)"
   using assms by (rel_auto, metis (full_types) vwb_lens_wb wb_lens.get_put)
 
 lemma seqr_insert_ident_left:
   assumes "vwb_lens x" "$x\<^sup>> \<sharp> P" "$x\<^sup>< \<sharp> Q"
-  shows "((($x\<^sup>> = $x\<^sup><)\<^sub>u \<and> P) ;; Q) = (P ;; Q)"
+  shows "((($x\<^sup>> = $x\<^sup><)\<^sub>u \<and> P) \<Zcomp> Q) = (P \<Zcomp> Q)"
   using assms by (rel_auto, meson vwb_lens_wb wb_lens_weak weak_lens.put_get)
 
 lemma seqr_insert_ident_right:
   assumes "vwb_lens x" "$x\<^sup>> \<sharp> P" "$x\<^sup>< \<sharp> Q"
-  shows "(P ;; (($x\<^sup>> = $x\<^sup><)\<^sub>u \<and> Q)) = (P ;; Q)"
-  using assms by (rel_auto, metis (no_types, hide_lams) vwb_lens_def wb_lens_def weak_lens.put_get)
+  shows "(P \<Zcomp> (($x\<^sup>> = $x\<^sup><)\<^sub>u \<and> Q)) = (P \<Zcomp> Q)"
+  using assms by (rel_auto, metis (no_types, opaque_lifting) vwb_lens_def wb_lens_def weak_lens.put_get)
 
 lemma seq_var_ident_lift:
   assumes "vwb_lens x" "$x\<^sup>> \<sharp> P" "$x\<^sup>< \<sharp> Q"
-  shows "((($x\<^sup>> = $x\<^sup><)\<^sub>u \<and> P) ;; (($x\<^sup>> = $x\<^sup><)\<^sub>u \<and> Q)) = (($x\<^sup>> = $x\<^sup><)\<^sub>u \<and> (P ;; Q))"
+  shows "((($x\<^sup>> = $x\<^sup><)\<^sub>u \<and> P) \<Zcomp> (($x\<^sup>> = $x\<^sup><)\<^sub>u \<and> Q)) = (($x\<^sup>> = $x\<^sup><)\<^sub>u \<and> (P \<Zcomp> Q))"
   using assms by (rel_auto, metis (no_types, lifting) vwb_lens_wb wb_lens_weak weak_lens.put_get)
 
 lemma seqr_bool_split:
   assumes "vwb_lens x"
-  shows "P ;; Q = (P\<lbrakk>true/x\<^sup>>\<rbrakk> ;; Q\<lbrakk>true/x\<^sup><\<rbrakk> \<or> P\<lbrakk>(false)\<^sub>u/x\<^sup>>\<rbrakk> ;; Q\<lbrakk>false/x\<^sup><\<rbrakk>)"
+  shows "P \<Zcomp> Q = (P\<lbrakk>true/x\<^sup>>\<rbrakk> \<Zcomp> Q\<lbrakk>true/x\<^sup><\<rbrakk> \<or> P\<lbrakk>(false)\<^sub>u/x\<^sup>>\<rbrakk> \<Zcomp> Q\<lbrakk>false/x\<^sup><\<rbrakk>)"
   using assms apply (subst seqr_middle[of x], simp_all)
   apply rel_auto
   oops
 
 lemma cond_inter_var_split:
   assumes "vwb_lens x"
-  shows "(P \<lhd> $x\<^sup>> \<rhd> Q) ;; R = (P\<lbrakk>true/x\<^sup>>\<rbrakk> ;; R\<lbrakk>true/x\<^sup><\<rbrakk> \<or> Q\<lbrakk>false/x\<^sup>>\<rbrakk> ;; R\<lbrakk>false/x\<^sup><\<rbrakk>)"
+  shows "(P \<lhd> $x\<^sup>> \<rhd> Q) \<Zcomp> R = (P\<lbrakk>true/x\<^sup>>\<rbrakk> \<Zcomp> R\<lbrakk>true/x\<^sup><\<rbrakk> \<or> Q\<lbrakk>false/x\<^sup>>\<rbrakk> \<Zcomp> R\<lbrakk>false/x\<^sup><\<rbrakk>)"
 proof -
-  have "(P \<lhd> $x\<^sup>> \<rhd> Q) ;; R = (((x\<^sup>>)\<^sub>u \<and> P) ;; R \<or> (\<not> (x\<^sup>>)\<^sub>u \<and> Q) ;; R)"
+  have "(P \<lhd> $x\<^sup>> \<rhd> Q) \<Zcomp> R = (((x\<^sup>>)\<^sub>u \<and> P) \<Zcomp> R \<or> (\<not> (x\<^sup>>)\<^sub>u \<and> Q) \<Zcomp> R)"
     by rel_simp
-  also have "... = ((P \<and> (x\<^sup>>)\<^sub>u) ;; R \<or> (Q \<and> \<not>(x\<^sup>>)\<^sub>u) ;; R)"
+  also have "... = ((P \<and> (x\<^sup>>)\<^sub>u) \<Zcomp> R \<or> (Q \<and> \<not>(x\<^sup>>)\<^sub>u) \<Zcomp> R)"
     by (rel_auto)
-  also have "... = (P\<lbrakk>true/x\<^sup>>\<rbrakk> ;; R\<lbrakk>true/x\<^sup><\<rbrakk> \<or> Q\<lbrakk>false/x\<^sup>>\<rbrakk> ;; R\<lbrakk>false/x\<^sup><\<rbrakk>)"
+  also have "... = (P\<lbrakk>true/x\<^sup>>\<rbrakk> \<Zcomp> R\<lbrakk>true/x\<^sup><\<rbrakk> \<or> Q\<lbrakk>false/x\<^sup>>\<rbrakk> \<Zcomp> R\<lbrakk>false/x\<^sup><\<rbrakk>)"
     apply (rel_auto add: seqr_left_one_point_true seqr_left_one_point_false assms)
     by (metis (full_types) assms vwb_lens_wb wb_lens.get_put)+
   finally show ?thesis .
 qed
 
-theorem seqr_pre_transfer: "in\<alpha> \<sharp> q \<Longrightarrow> ((P \<and> q) ;; R) = (P ;; (q\<^sup>- \<and> R))"
+theorem seqr_pre_transfer: "in\<alpha> \<sharp> q \<Longrightarrow> ((P \<and> q) \<Zcomp> R) = (P \<Zcomp> (q\<^sup>- \<and> R))"
   by rel_auto
 
 theorem seqr_pre_transfer':
-  "((P \<and> (q\<^sup>>)\<^sub>u) ;; R) = (P ;; ((q\<^sup><)\<^sub>u \<and> R))"
+  "((P \<and> (q\<^sup>>)\<^sub>u) \<Zcomp> R) = (P \<Zcomp> ((q\<^sup><)\<^sub>u \<and> R))"
   by (rel_auto)
 
-theorem seqr_post_out: "in\<alpha> \<sharp> r \<Longrightarrow> (P ;; (Q \<and> r)) = ((P ;; Q) \<and> r)"
+theorem seqr_post_out: "in\<alpha> \<sharp> r \<Longrightarrow> (P \<Zcomp> (Q \<and> r)) = ((P \<Zcomp> Q) \<and> r)"
   by (rel_auto)
 
 lemma seqr_post_var_out:
-  shows "(P ;; (Q \<and> (x\<^sup>>)\<^sub>u)) = ((P ;; Q) \<and> (x\<^sup>>)\<^sub>u)"
+  shows "(P \<Zcomp> (Q \<and> (x\<^sup>>)\<^sub>u)) = ((P \<Zcomp> Q) \<and> (x\<^sup>>)\<^sub>u)"
   by (rel_auto)
 
-theorem seqr_post_transfer: "out\<alpha> \<sharp> q \<Longrightarrow> (P ;; (q \<and> R)) = ((P \<and> q\<^sup>-) ;; R)"
+theorem seqr_post_transfer: "out\<alpha> \<sharp> q \<Longrightarrow> (P \<Zcomp> (q \<and> R)) = ((P \<and> q\<^sup>-) \<Zcomp> R)"
   by (rel_auto)
 
-lemma seqr_pre_out: "out\<alpha> \<sharp> p \<Longrightarrow> ((p \<and> Q) ;; R) = (p \<and> (Q ;; R))"
+lemma seqr_pre_out: "out\<alpha> \<sharp> p \<Longrightarrow> ((p \<and> Q) \<Zcomp> R) = (p \<and> (Q \<Zcomp> R))"
   by (rel_auto)
 
 lemma seqr_pre_var_out:
-  shows "(((x\<^sup><)\<^sub>u \<and> P) ;; Q) = ((x\<^sup><)\<^sub>u \<and> (P ;; Q))"
+  shows "(((x\<^sup><)\<^sub>u \<and> P) \<Zcomp> Q) = ((x\<^sup><)\<^sub>u \<and> (P \<Zcomp> Q))"
   by (rel_auto)
 
 lemma seqr_true_lemma:
-  "(P = (\<not> ((\<not> P) ;; true))) = (P = (P ;; true))"
+  "(P = (\<not> ((\<not> P) \<Zcomp> true))) = (P = (P \<Zcomp> true))"
   by (rel_auto)
 
-lemma seqr_to_conj: "\<lbrakk> out\<alpha> \<sharp> P; in\<alpha> \<sharp> Q \<rbrakk> \<Longrightarrow> (P ;; Q) = (P \<and> Q)"
+lemma seqr_to_conj: "\<lbrakk> out\<alpha> \<sharp> P; in\<alpha> \<sharp> Q \<rbrakk> \<Longrightarrow> (P \<Zcomp> Q) = (P \<and> Q)"
   by (rel_auto; blast)
 
 lemma liberate_seq_unfold:
-  "vwb_lens x \<Longrightarrow> $x \<sharp> Q \<Longrightarrow> (P \\ $x) ;; Q = (P ;; Q) \\ $x"
+  "vwb_lens x \<Longrightarrow> $x \<sharp> Q \<Longrightarrow> (P \\ $x) \<Zcomp> Q = (P \<Zcomp> Q) \\ $x"
   apply (rel_auto add: liberate_pred_def)
   oops
 
 (*
 lemma shEx_mem_lift_seq_1 [uquant_lift]:
   assumes "out\<alpha> \<sharp> A"
-  shows "((\<^bold>\<exists> x \<in> A \<bullet> P x) ;; Q) = (\<^bold>\<exists> x \<in> A \<bullet> (P x ;; Q))"
+  shows "((\<^bold>\<exists> x \<in> A \<bullet> P x) \<Zcomp> Q) = (\<^bold>\<exists> x \<in> A \<bullet> (P x \<Zcomp> Q))"
   using assms by rel_blast
 
 lemma shEx_lift_seq_2 [uquant_lift]:
-  "(P ;; (\<^bold>\<exists> x \<bullet> Q x)) = (\<^bold>\<exists> x \<bullet> (P ;; Q x))"
+  "(P \<Zcomp> (\<^bold>\<exists> x \<bullet> Q x)) = (\<^bold>\<exists> x \<bullet> (P \<Zcomp> Q x))"
   by rel_auto
 
 lemma shEx_mem_lift_seq_2 [uquant_lift]:
   assumes "in\<alpha> \<sharp> A"
-  shows "(P ;; (\<^bold>\<exists> x \<in> A \<bullet> Q x)) = (\<^bold>\<exists> x \<in> A \<bullet> (P ;; Q x))"
+  shows "(P \<Zcomp> (\<^bold>\<exists> x \<in> A \<bullet> Q x)) = (\<^bold>\<exists> x \<in> A \<bullet> (P \<Zcomp> Q x))"
   using assms by rel_blast*)
 
 subsection \<open> Iterated Sequential Composition Laws \<close>
   
-lemma iter_seqr_nil [simp]: "(;; i : [] \<bullet> P(i)) = II"
+lemma iter_seqr_nil [simp]: "(\<Zcomp> i : [] \<bullet> P(i)) = II"
   by (simp add: seqr_iter_def)
     
-lemma iter_seqr_cons [simp]: "(;; i : (x # xs) \<bullet> P(i)) = P(x) ;; (;; i : xs \<bullet> P(i))"
+lemma iter_seqr_cons [simp]: "(\<Zcomp> i : (x # xs) \<bullet> P(i)) = P(x) \<Zcomp> (\<Zcomp> i : xs \<bullet> P(i))"
   by (simp add: seqr_iter_def)
 
 subsection \<open> Quantale Laws \<close>
@@ -244,28 +250,28 @@ subsection \<open> Quantale Laws \<close>
 text \<open> Kept here for backwards compatibility, remove when this library catches up with the old UTP
        as most of these are already proven in Relation.thy\<close>
 
-lemma seq_Sup_distl: "P ;; (\<Union> A) = (\<Union> Q\<in>A. P ;; Q)"
+lemma seq_Sup_distl: "P \<Zcomp> (\<Union> A) = (\<Union> Q\<in>A. P \<Zcomp> Q)"
   by (transfer, auto)
 
-lemma seq_Sup_distr: "(\<Union> A) ;; Q = (\<Union> P\<in>A. P ;; Q)"
+lemma seq_Sup_distr: "(\<Union> A) \<Zcomp> Q = (\<Union> P\<in>A. P \<Zcomp> Q)"
   by (transfer, auto)
 
-lemma seq_UINF_distl: "P ;; (\<Union> Q\<in>A. F(Q)) = (\<Union> Q\<in>A. P ;; F(Q))"
+lemma seq_UINF_distl: "P \<Zcomp> (\<Union> Q\<in>A. F(Q)) = (\<Union> Q\<in>A. P \<Zcomp> F(Q))"
   by auto
 
-lemma seq_UINF_distl': "P ;; (\<Union> Q. F(Q)) = (\<Union> Q. P ;; F(Q))"
+lemma seq_UINF_distl': "P \<Zcomp> (\<Union> Q. F(Q)) = (\<Union> Q. P \<Zcomp> F(Q))"
   by (metis seq_UINF_distl)
 
-lemma seq_UINF_distr: "(\<Union> P\<in>A . F(P)) ;; Q = (\<Union> P\<in>A. F(P) ;; Q)"
+lemma seq_UINF_distr: "(\<Union> P\<in>A . F(P)) \<Zcomp> Q = (\<Union> P\<in>A. F(P) \<Zcomp> Q)"
   by auto
 
-lemma seq_UINF_distr': "(\<Union> P. F(P)) ;; Q = (\<Union> P. F(P) ;; Q)"
+lemma seq_UINF_distr': "(\<Union> P. F(P)) \<Zcomp> Q = (\<Union> P. F(P) \<Zcomp> Q)"
   by (metis seq_UINF_distr)
 
-lemma seq_SUP_distl: "P ;; (\<Union>i\<in>A. Q(i)) = (\<Union>i\<in>A. P ;; Q(i))"
+lemma seq_SUP_distl: "P \<Zcomp> (\<Union>i\<in>A. Q(i)) = (\<Union>i\<in>A. P \<Zcomp> Q(i))"
   by (metis image_image seq_Sup_distl)
 
-lemma seq_SUP_distr: "(\<Union>i\<in>A. P(i)) ;; Q = (\<Union>i\<in>A. P(i) ;; Q)"
+lemma seq_SUP_distr: "(\<Union>i\<in>A. P(i)) \<Zcomp> Q = (\<Union>i\<in>A. P(i) \<Zcomp> Q)"
   by (simp add: seq_Sup_distr)
 
 subsection \<open> Skip Laws \<close>
@@ -305,20 +311,23 @@ lemma skip_res_as_ra:
   done
 *)
 subsection \<open> Assignment Laws \<close>
-  
-lemma assigns_subst [usubst]:
-  "\<lceil>\<sigma>\<rceil>\<^sub>s \<dagger> \<langle>\<rho>\<rangle>\<^sub>a = \<langle>\<rho> \<circ>\<^sub>s \<sigma>\<rangle>\<^sub>a"
-  by (rel_auto)
 
-lemma assigns_r_comp: "(\<langle>\<sigma>\<rangle>\<^sub>a ;; P) = (\<lceil>\<sigma>\<rceil>\<^sub>s \<dagger> P)"
+text \<open>Extend the alphabet of a substitution\<close>
+definition subst_aext :: "'a subst \<Rightarrow> ('a \<Longrightarrow> 'b) \<Rightarrow> 'b subst"
+  where [rel]: "subst_aext \<sigma> x = (\<lambda> s. put\<^bsub>x\<^esub> s (\<sigma> (get\<^bsub>x\<^esub> s)))"
+
+lemma assigns_subst: "(subst_aext \<sigma> fst\<^sub>L) \<dagger> \<langle>\<rho>\<rangle>\<^sub>a = \<langle>\<rho> \<circ>\<^sub>s \<sigma>\<rangle>\<^sub>a"
+  by rel_auto
+
+lemma assigns_r_comp: "(\<langle>\<sigma>\<rangle>\<^sub>a \<Zcomp> P) = ((\<lambda> s. put\<^bsub>fst\<^sub>L\<^esub> s (\<sigma> (get\<^bsub>fst\<^sub>L\<^esub> s))) \<dagger> P)"
   by (rel_auto)
 
 lemma assigns_r_feasible:
-  "(\<langle>\<sigma>\<rangle>\<^sub>a ;; true) = true"
+  "(\<langle>\<sigma>\<rangle>\<^sub>a \<Zcomp> true) = true"
   by (rel_auto)
 
 lemma assign_subst [usubst]:
-  "\<lbrakk> mwb_lens x; mwb_lens y \<rbrakk> \<Longrightarrow> [$x \<mapsto>\<^sub>s \<lceil>u\<rceil>\<^sub><] \<dagger> (y := v) = (x, y) := (u, [x \<mapsto>\<^sub>s u] \<dagger> v)"
+  "\<lbrakk> mwb_lens x; mwb_lens y \<rbrakk> \<Longrightarrow> [x \<leadsto> u\<^sup><] \<dagger> (y := v) = (x, y) := (u, [x \<leadsto> u] \<dagger> v)"
   by (rel_auto)
 
 lemma assign_vacuous_skip:
@@ -331,7 +340,7 @@ text \<open> The following law shows the case for the above law when $x$ is only
 
 lemma assign_vacuous_assume:
   assumes "mwb_lens x"
-  shows "[&\<^bold>v \<in> \<guillemotleft>\<S>\<^bsub>x\<^esub>\<guillemotright>]\<^sup>\<top> ;; (x := &x) = [&\<^bold>v \<in> \<guillemotleft>\<S>\<^bsub>x\<^esub>\<guillemotright>]\<^sup>\<top>"
+  shows "[&\<^bold>v \<in> \<guillemotleft>\<S>\<^bsub>x\<^esub>\<guillemotright>]\<^sup>\<top> \<Zcomp> (x := &x) = [&\<^bold>v \<in> \<guillemotleft>\<S>\<^bsub>x\<^esub>\<guillemotright>]\<^sup>\<top>"
   using assms by rel_auto
 
 lemma assign_simultaneous:
@@ -354,29 +363,29 @@ lemma assign_pred_transfer:
   shows "(b \<and> x := v) = (x := v \<and> b\<^sup>-)"
   using assms apply rel_auto oops
     
-lemma assign_r_comp: "x := u ;; P = P\<lbrakk>u\<^sup></x\<^sup><\<rbrakk>"
+lemma assign_r_comp: "x := u \<Zcomp> P = P\<lbrakk>u\<^sup></x\<^sup><\<rbrakk>"
   by rel_auto
 
-lemma assign_test: "mwb_lens x \<Longrightarrow> (x := \<guillemotleft>u\<guillemotright> ;; x := \<guillemotleft>v\<guillemotright>) = (x := \<guillemotleft>v\<guillemotright>)"
+lemma assign_test: "mwb_lens x \<Longrightarrow> (x := \<guillemotleft>u\<guillemotright> \<Zcomp> x := \<guillemotleft>v\<guillemotright>) = (x := \<guillemotleft>v\<guillemotright>)"
   by rel_auto
 
-lemma assign_twice: "\<lbrakk> mwb_lens x; $x \<sharp> f \<rbrakk> \<Longrightarrow> (x := e ;; x := f) = (x := f)"
+lemma assign_twice: "\<lbrakk> mwb_lens x; $x \<sharp> f \<rbrakk> \<Longrightarrow> (x := e \<Zcomp> x := f) = (x := f)"
   by rel_auto
  
 lemma assign_commute:
   assumes "x \<bowtie> y" "$x \<sharp> f" "$y \<sharp> e" "vwb_lens x" "vwb_lens y"
-  shows "(x := e ;; y := f) = (y := f ;; x := e)"
+  shows "(x := e \<Zcomp> y := f) = (y := f \<Zcomp> x := e)"
   using assms by (rel_auto add: lens_indep_comm)
 
 lemma assign_cond:
   fixes x :: "('a \<Longrightarrow> '\<alpha>)"
   assumes "out\<alpha> \<sharp> b"
-  shows "(x := e ;; (P \<triangleleft> b \<triangleright> Q)) = ((x := e ;; P) \<triangleleft> b \<triangleright> (x := e ;; Q))"
+  shows "(x := e \<Zcomp> (P \<triangleleft> b \<triangleright> Q)) = ((x := e \<Zcomp> P) \<triangleleft> b \<triangleright> (x := e \<Zcomp> Q))"
   by (rel_auto)
 
 lemma assign_rcond:
   fixes x :: "('a \<Longrightarrow> '\<alpha>)"
-  shows "(x := e ;; (P \<triangleleft> b \<triangleright>\<^sub>r Q)) = ((x := e ;; P) \<triangleleft> (b\<lbrakk>e/x\<rbrakk>) \<triangleright>\<^sub>r (x := e ;; Q))"
+  shows "(x := e \<Zcomp> (P \<^bold>\<lhd> b \<^bold>\<rhd> Q)) = ((x := e \<Zcomp> P) \<triangleleft> (b\<lbrakk>e/x\<rbrakk>) \<triangleright>\<^sub>r (x := e \<Zcomp> Q))"
   by (rel_auto)
 
 lemma assign_r_alt_def:
@@ -402,11 +411,11 @@ lemma assign_unfold:
 subsection \<open> Non-deterministic Assignment Laws \<close>
 
 lemma nd_assign_comp:
-  "x \<bowtie> y \<Longrightarrow> x := * ;; y := * = (x,y) := *"
+  "x \<bowtie> y \<Longrightarrow> x := * \<Zcomp> y := * = (x,y) := *"
   apply (rel_auto) using lens_indep_comm sorry
 
 lemma nd_assign_assign:
-  "\<lbrakk> vwb_lens x; x \<sharp> e \<rbrakk> \<Longrightarrow> x := * ;; x := e = x := e"
+  "\<lbrakk> vwb_lens x; x \<sharp> e \<rbrakk> \<Longrightarrow> x := * \<Zcomp> x := e = x := e"
   by (rel_auto)
 
 subsection \<open> Converse Laws \<close>
@@ -445,7 +454,7 @@ lemma disj_convr [simp]: "(p \<or> q)\<^sup>- = (q\<^sup>- \<or> p\<^sup>-)"
 lemma conj_convr [simp]: "(p \<and> q)\<^sup>- = (q\<^sup>- \<and> p\<^sup>-)"
   by (pred_auto)
 
-lemma seqr_convr [simp]: "(p ;; q)\<^sup>- = (q\<^sup>- ;; p\<^sup>-)"
+lemma seqr_convr [simp]: "(p \<Zcomp> q)\<^sup>- = (q\<^sup>- \<Zcomp> p\<^sup>-)"
   by (rel_auto)
 
 lemma pre_convr [simp]: "\<lceil>p\<rceil>\<^sub><\<^sup>- = \<lceil>p\<rceil>\<^sub>>"
@@ -464,7 +473,7 @@ lemma assume_false: "[false]\<^sup>\<top> = false"
 lemma assume_true: "[true]\<^sup>\<top> = II"
   by (rel_auto)
     
-lemma assume_seq: "[b]\<^sup>\<top> ;; [c]\<^sup>\<top> = [(b \<and> c)]\<^sup>\<top>"
+lemma assume_seq: "[b]\<^sup>\<top> \<Zcomp> [c]\<^sup>\<top> = [(b \<and> c)]\<^sup>\<top>"
   by (rel_auto)
 
 lemma assert_false: "{false}\<^sub>\<bottom> = true"
@@ -473,21 +482,21 @@ lemma assert_false: "{false}\<^sub>\<bottom> = true"
 lemma assert_true: "{true}\<^sub>\<bottom> = II"
   by (rel_auto)
     
-lemma assert_seq: "{b}\<^sub>\<bottom> ;; {c}\<^sub>\<bottom> = {(b \<and> c)}\<^sub>\<bottom>"
+lemma assert_seq: "{b}\<^sub>\<bottom> \<Zcomp> {c}\<^sub>\<bottom> = {(b \<and> c)}\<^sub>\<bottom>"
   by (rel_auto)
 
 subsection \<open> While Loop Laws \<close>
 
 theorem while_unfold:
-  "while b do P od = ((P ;; while b do P od) \<Zdres> b \<Zrres> II)"
+  "while b do P od = ((P \<Zcomp> while b do P od) \<^bold>\<lhd> b \<^bold>\<rhd> II)"
 proof -
-  have m:"mono (\<lambda>X. (P ;; X) \<triangleleft> b \<triangleright>\<^sub>r II)"
-    by (auto intro: monoI seqr_mono cond_mono)
-  have "(while b do P od) = (\<nu> X \<bullet> (P ;; X) \<triangleleft> b \<triangleright>\<^sub>r II)"
+  have m:"mono (\<lambda>X. (P \<Zcomp> X) \<^bold>\<lhd> b \<^bold>\<rhd> II)"
+    unfolding mono_def by (meson equalityE rcond_mono ref_by_def relcomp_mono)
+  have "(while b do P od) = (\<nu> X \<bullet> (P \<Zcomp> X) \<^bold>\<lhd> b \<^bold>\<rhd> II)"
     by (simp add: while_top_def)
-  also have "... = ((P ;; (\<nu> X \<bullet> (P ;; X) \<triangleleft> b \<triangleright>\<^sub>r II)) \<triangleleft> b \<triangleright>\<^sub>r II)"
+  also have "... = ((P \<Zcomp> (\<nu> X \<bullet> (P \<Zcomp> X) \<^bold>\<lhd> b \<^bold>\<rhd> II)) \<^bold>\<lhd> b \<^bold>\<rhd> II)"
     by (subst lfp_unfold, simp_all add: m)
-  also have "... = ((P ;; while b do P od) \<triangleleft> b \<triangleright>\<^sub>r II)"
+  also have "... = ((P \<Zcomp> while b do P od) \<^bold>\<lhd> b \<^bold>\<rhd> II)"
     by (simp add: while_top_def)
   finally show ?thesis .
 qed
@@ -495,60 +504,57 @@ qed
 theorem while_false: "while (false)\<^sub>e do P od = II"
   by (subst while_unfold, rel_auto)
 
-theorem while_true: "while true do P od = false"
+theorem while_true: "while (true)\<^sub>e do P od = false"
   apply (simp add: while_top_def alpha)
   apply (rule antisym)
-   apply (simp_all)
   apply (rule lfp_lowerbound)
-  apply (rel_auto)
+  apply (rel_auto)+
   done
 
 theorem while_bot_unfold:
-  "while\<^sub>\<bottom> b do P od = ((P ;; while\<^sub>\<bottom> b do P od) \<triangleleft> b \<triangleright>\<^sub>r II)"
+  "while\<^sub>\<bottom> b do P od = ((P \<Zcomp> while\<^sub>\<bottom> b do P od) \<^bold>\<lhd> b \<^bold>\<rhd> II)"
 proof -
-  have m:"mono (\<lambda>X. (P ;; X) \<triangleleft> b \<triangleright>\<^sub>r II)"
-    by (auto intro: monoI seqr_mono cond_mono)
-  have "(while\<^sub>\<bottom> b do P od) = (\<mu> X \<bullet> (P ;; X) \<triangleleft> b \<triangleright>\<^sub>r II)"
+  have m:"mono (\<lambda>X. (P \<Zcomp> X) \<^bold>\<lhd> b \<^bold>\<rhd> II)"
+    unfolding mono_def by (meson equalityE rcond_mono ref_by_def relcomp_mono)
+  have "(while\<^sub>\<bottom> b do P od) = (\<mu> X \<bullet> (P \<Zcomp> X) \<^bold>\<lhd> b \<^bold>\<rhd> II)"
     by (simp add: while_bot_def)
-  also have "... = ((P ;; (\<mu> X \<bullet> (P ;; X) \<triangleleft> b \<triangleright>\<^sub>r II)) \<triangleleft> b \<triangleright>\<^sub>r II)"
+  also have "... = ((P \<Zcomp> (\<mu> X \<bullet> (P \<Zcomp> X) \<^bold>\<lhd> b \<^bold>\<rhd> II)) \<^bold>\<lhd> b \<^bold>\<rhd> II)"
     by (subst gfp_unfold, simp_all add: m)
-  also have "... = ((P ;; while\<^sub>\<bottom> b do P od) \<triangleleft> b \<triangleright>\<^sub>r II)"
+  also have "... = ((P \<Zcomp> while\<^sub>\<bottom> b do P od) \<^bold>\<lhd> b \<^bold>\<rhd> II)"
     by (simp add: while_bot_def)
   finally show ?thesis .
 qed
 
-theorem while_bot_false: "while\<^sub>\<bottom> false do P od = II"
+theorem while_bot_false: "while\<^sub>\<bottom> (false)\<^sub>e do P od = II"
   by (simp add: while_bot_def mu_const alpha)
 
-theorem while_bot_true: "while\<^sub>\<bottom> true do P od = (\<mu> X \<bullet> P ;; X)"
+theorem while_bot_true: "while\<^sub>\<bottom> (true)\<^sub>e do P od = (\<mu> X \<bullet> P \<Zcomp> X)"
   by (simp add: while_bot_def alpha)
 
 text \<open> An infinite loop with a feasible body corresponds to a program error (non-termination). \<close>
 
-theorem while_infinite: "P ;; true\<^sub>h = true \<Longrightarrow> while\<^sub>\<bottom> true do P od = true"
+theorem while_infinite: "P \<Zcomp> true = true \<Longrightarrow> while\<^sub>\<bottom> (true)\<^sub>e do P od = true"
   apply (simp add: while_bot_true)
   apply (rule antisym)
-   apply (simp)
+  apply (simp add: true_pred_def)
   apply (rule gfp_upperbound)
-  apply (simp)
+  apply (rel_auto)
   done
 
 subsection \<open> Algebraic Properties \<close>
 
-interpretation upred_semiring: semiring_1
-  where times = seqr and one = skip_r and zero = false\<^sub>h and plus = Lattices.sup
-  by (unfold_locales, (rel_auto)+)
+interpretation upred_semiring: semiring_1 uskip useq "(\<union>)" "{}"
 
 declare upred_semiring.power_Suc [simp del]
 
 text \<open> We introduce the power syntax derived from semirings \<close>
 
-abbreviation upower :: "'\<alpha> hrel \<Rightarrow> nat \<Rightarrow> '\<alpha> hrel" (infixr "\<^bold>^" 80) where
+abbreviation upower :: "'\<alpha> rel \<Rightarrow> nat \<Rightarrow> '\<alpha> rel" (infixr "\<^bold>^" 80) where
 "upower P n \<equiv> upred_semiring.power P n"
 
 translations
-  "P \<^bold>^ i" <= "CONST power.power II op ;; P i"
-  "P \<^bold>^ i" <= "(CONST power.power II op ;; P) i"
+  "P \<^bold>^ i" <= "CONST power.power II op \<Zcomp> P i"
+  "P \<^bold>^ i" <= "(CONST power.power II op \<Zcomp> P) i"
 
 text \<open> Set up transfer tactic for powers \<close>
 
@@ -565,7 +571,7 @@ next
 qed
 
 lemma upower_rep_eq_alt:
-  "\<lbrakk>power.power \<langle>id\<^sub>s\<rangle>\<^sub>a (;;) P i\<rbrakk>\<^sub>e = (\<lambda>b. b \<in> ({p. \<lbrakk>P\<rbrakk>\<^sub>e p} ^^ i))"
+  "\<lbrakk>power.power \<langle>id\<^sub>s\<rangle>\<^sub>a (\<Zcomp>) P i\<rbrakk>\<^sub>e = (\<lambda>b. b \<in> ({p. \<lbrakk>P\<rbrakk>\<^sub>e p} ^^ i))"
   by (metis skip_r_def upower_rep_eq)
 
 update_uexpr_rep_eq_thms
@@ -600,7 +606,7 @@ text \<open> The following two proofs are adapted from the AFP entry
   \href{https://www.isa-afp.org/entries/Kleene_Algebra.shtml}{Kleene Algebra}. 
   See also~\cite{Armstrong2012,Armstrong2015}. \<close>
 
-lemma upower_inductl: "Q \<sqsubseteq> ((P ;; Q) \<sqinter> R) \<Longrightarrow> Q \<sqsubseteq> P \<^bold>^ n ;; R"
+lemma upower_inductl: "Q \<sqsubseteq> ((P \<Zcomp> Q) \<sqinter> R) \<Longrightarrow> Q \<sqsubseteq> P \<^bold>^ n \<Zcomp> R"
 proof (induct n)
   case 0
   then show ?case by (auto)
@@ -611,16 +617,16 @@ next
 qed
 
 lemma upower_inductr:
-  assumes "Q \<sqsubseteq> R \<sqinter> (Q ;; P)"
-  shows "Q \<sqsubseteq> R ;; (P \<^bold>^ n)"
+  assumes "Q \<sqsubseteq> R \<sqinter> (Q \<Zcomp> P)"
+  shows "Q \<sqsubseteq> R \<Zcomp> (P \<^bold>^ n)"
 using assms proof (induct n)
   case 0
   then show ?case by auto
 next
   case (Suc n)
-  have "R ;; P \<^bold>^ Suc n = (R ;; P \<^bold>^ n) ;; P"
+  have "R \<Zcomp> P \<^bold>^ Suc n = (R \<Zcomp> P \<^bold>^ n) \<Zcomp> P"
     by (metis seqr_assoc upred_semiring.power_Suc2)
-  also have "Q ;; P \<sqsubseteq> ..."
+  also have "Q \<Zcomp> P \<sqsubseteq> ..."
     by (meson Suc.hyps assms eq_iff seqr_mono)
   also have "Q \<sqsubseteq> ..."
     using assms by auto
@@ -633,7 +639,7 @@ lemma SUP_atLeastAtMost_first:
   shows "(\<Sqinter>i\<in>{m..n}. P(i)) = P(m) \<sqinter> (\<Sqinter>i\<in>{Suc m..n}. P(i))"
   by (metis SUP_insert assms atLeastAtMost_insertL)
     
-lemma upower_seqr_iter: "P \<^bold>^ n = (;; Q : replicate n P \<bullet> Q)"
+lemma upower_seqr_iter: "P \<^bold>^ n = (\<Zcomp> Q : replicate n P \<bullet> Q)"
   by (induct n, simp_all add: upred_semiring.power_Suc)
 
 lemma assigns_power: "\<langle>f\<rangle>\<^sub>a \<^bold>^ n = \<langle>f ^\<^sub>s n\<rangle>\<^sub>a"
@@ -641,7 +647,7 @@ lemma assigns_power: "\<langle>f\<rangle>\<^sub>a \<^bold>^ n = \<langle>f ^\<^s
 
 subsection \<open> Kleene Star \<close>
 
-definition ustar :: "'\<alpha> hrel \<Rightarrow> '\<alpha> hrel" ("_\<^sup>\<star>" [999] 999) where
+definition ustar :: "'\<alpha> rel \<Rightarrow> '\<alpha> rel" ("_\<^sup>\<star>" [999] 999) where
 "P\<^sup>\<star> = (\<Sqinter>i\<in>{0..} \<bullet> P\<^bold>^i)"
 
 lemma ustar_rep_eq:
@@ -654,38 +660,38 @@ subsection \<open> Kleene Plus \<close>
 
 purge_notation trancl ("(_\<^sup>+)" [1000] 999)
 
-definition uplus :: "'\<alpha> hrel \<Rightarrow> '\<alpha> hrel" ("_\<^sup>+" [999] 999) where
-[upred_defs]: "P\<^sup>+ = P ;; P\<^sup>\<star>"
+definition uplus :: "'\<alpha> rel \<Rightarrow> '\<alpha> rel" ("_\<^sup>+" [999] 999) where
+[upred_defs]: "P\<^sup>+ = P \<Zcomp> P\<^sup>\<star>"
 
 lemma uplus_power_def: "P\<^sup>+ = (\<Sqinter> i \<bullet> P \<^bold>^ (Suc i))"
   by (simp add: uplus_def ustar_def seq_UINF_distl' UINF_atLeast_Suc upred_semiring.power_Suc)
 
 subsection \<open> Omega \<close>
 
-definition uomega :: "'\<alpha> hrel \<Rightarrow> '\<alpha> hrel" ("_\<^sup>\<omega>" [999] 999) where
-"P\<^sup>\<omega> = (\<mu> X \<bullet> P ;; X)"
+definition uomega :: "'\<alpha> rel \<Rightarrow> '\<alpha> rel" ("_\<^sup>\<omega>" [999] 999) where
+"P\<^sup>\<omega> = (\<mu> X \<bullet> P \<Zcomp> X)"
 
 subsection \<open> Relation Algebra Laws \<close>
 
-theorem RA1: "(P ;; (Q ;; R)) = ((P ;; Q) ;; R)"
+theorem RA1: "(P \<Zcomp> (Q \<Zcomp> R)) = ((P \<Zcomp> Q) \<Zcomp> R)"
   by (simp add: seqr_assoc)
 
-theorem RA2: "(P ;; II) = P" "(II ;; P) = P"
+theorem RA2: "(P \<Zcomp> II) = P" "(II \<Zcomp> P) = P"
   by simp_all
 
 theorem RA3: "P\<^sup>-\<^sup>- = P"
   by simp
 
-theorem RA4: "(P ;; Q)\<^sup>- = (Q\<^sup>- ;; P\<^sup>-)"
+theorem RA4: "(P \<Zcomp> Q)\<^sup>- = (Q\<^sup>- \<Zcomp> P\<^sup>-)"
   by simp
 
 theorem RA5: "(P \<or> Q)\<^sup>- = (P\<^sup>- \<or> Q\<^sup>-)"
   by (rel_auto)
 
-theorem RA6: "((P \<or> Q) ;; R) = (P;;R \<or> Q;;R)"
+theorem RA6: "((P \<or> Q) \<Zcomp> R) = (P\<Zcomp>R \<or> Q\<Zcomp>R)"
   using seqr_or_distl by blast
 
-theorem RA7: "((P\<^sup>- ;; (\<not>(P ;; Q))) \<or> (\<not>Q)) = (\<not>Q)"
+theorem RA7: "((P\<^sup>- \<Zcomp> (\<not>(P \<Zcomp> Q))) \<or> (\<not>Q)) = (\<not>Q)"
   by (rel_auto)
 
 subsection \<open> Kleene Algebra Laws \<close>
@@ -693,14 +699,14 @@ subsection \<open> Kleene Algebra Laws \<close>
 lemma ustar_alt_def: "P\<^sup>\<star> = (\<Sqinter> i \<bullet> P \<^bold>^ i)"
   by (simp add: ustar_def)
 
-theorem ustar_sub_unfoldl: "P\<^sup>\<star> \<sqsubseteq> II \<sqinter> (P;;P\<^sup>\<star>)"
+theorem ustar_sub_unfoldl: "P\<^sup>\<star> \<sqsubseteq> II \<sqinter> (P\<Zcomp>P\<^sup>\<star>)"
   by (rel_simp, simp add: rtrancl_into_trancl2 trancl_into_rtrancl)
     
 theorem ustar_inductl:
-  assumes "Q \<sqsubseteq> R" "Q \<sqsubseteq> P ;; Q"
-  shows "Q \<sqsubseteq> P\<^sup>\<star> ;; R"
+  assumes "Q \<sqsubseteq> R" "Q \<sqsubseteq> P \<Zcomp> Q"
+  shows "Q \<sqsubseteq> P\<^sup>\<star> \<Zcomp> R"
 proof -
-  have "P\<^sup>\<star> ;; R = (\<Sqinter> i. P \<^bold>^ i ;; R)"
+  have "P\<^sup>\<star> \<Zcomp> R = (\<Sqinter> i. P \<^bold>^ i \<Zcomp> R)"
     by (simp add: ustar_def UINF_as_Sup_collect' seq_SUP_distr)
   also have "Q \<sqsubseteq> ..."
     by (simp add: SUP_least assms upower_inductl)
@@ -708,30 +714,30 @@ proof -
 qed
 
 theorem ustar_inductr:
-  assumes "Q \<sqsubseteq> R" "Q \<sqsubseteq> Q ;; P"
-  shows "Q \<sqsubseteq> R ;; P\<^sup>\<star>"
+  assumes "Q \<sqsubseteq> R" "Q \<sqsubseteq> Q \<Zcomp> P"
+  shows "Q \<sqsubseteq> R \<Zcomp> P\<^sup>\<star>"
 proof -
-  have "R ;; P\<^sup>\<star> = (\<Sqinter> i. R ;; P \<^bold>^ i)"
+  have "R \<Zcomp> P\<^sup>\<star> = (\<Sqinter> i. R \<Zcomp> P \<^bold>^ i)"
     by (simp add: ustar_def UINF_as_Sup_collect' seq_SUP_distl)
   also have "Q \<sqsubseteq> ..."
     by (simp add: SUP_least assms upower_inductr)
   finally show ?thesis .
 qed
 
-lemma ustar_refines_nu: "(\<nu> X \<bullet> (P ;; X) \<sqinter> II) \<sqsubseteq> P\<^sup>\<star>"
+lemma ustar_refines_nu: "(\<nu> X \<bullet> (P \<Zcomp> X) \<sqinter> II) \<sqsubseteq> P\<^sup>\<star>"
   by (metis (no_types, lifting) lfp_greatest semilattice_sup_class.le_sup_iff 
       semilattice_sup_class.sup_idem upred_semiring.mult_2_right 
       upred_semiring.one_add_one ustar_inductl)
 
-lemma ustar_as_nu: "P\<^sup>\<star> = (\<nu> X \<bullet> (P ;; X) \<sqinter> II)"
+lemma ustar_as_nu: "P\<^sup>\<star> = (\<nu> X \<bullet> (P \<Zcomp> X) \<sqinter> II)"
 proof (rule antisym)
-  show "(\<nu> X \<bullet> (P ;; X) \<sqinter> II) \<sqsubseteq> P\<^sup>\<star>"
+  show "(\<nu> X \<bullet> (P \<Zcomp> X) \<sqinter> II) \<sqsubseteq> P\<^sup>\<star>"
     by (simp add: ustar_refines_nu)
-  show "P\<^sup>\<star> \<sqsubseteq> (\<nu> X \<bullet> (P ;; X) \<sqinter> II)"
+  show "P\<^sup>\<star> \<sqsubseteq> (\<nu> X \<bullet> (P \<Zcomp> X) \<sqinter> II)"
     by (metis lfp_lowerbound upred_semiring.add_commute ustar_sub_unfoldl)
 qed
 
-lemma ustar_unfoldl: "P\<^sup>\<star> = II \<sqinter> (P ;; P\<^sup>\<star>)"
+lemma ustar_unfoldl: "P\<^sup>\<star> = II \<sqinter> (P \<Zcomp> P\<^sup>\<star>)"
   apply (simp add: ustar_as_nu)
   apply (subst lfp_unfold)
    apply (rule monoI)
@@ -741,20 +747,20 @@ lemma ustar_unfoldl: "P\<^sup>\<star> = II \<sqinter> (P ;; P\<^sup>\<star>)"
 text \<open> While loop can be expressed using Kleene star \<close>
 
 lemma while_star_form:
-  "while b do P od = (P \<triangleleft> b \<triangleright>\<^sub>r II)\<^sup>\<star> ;; [(\<not>b)]\<^sup>\<top>"
+  "while b do P od = (P \<^bold>\<lhd> b \<^bold>\<rhd> II)\<^sup>\<star> \<Zcomp> [(\<not>b)]\<^sup>\<top>"
 proof -
-  have 1: "Continuous (\<lambda>X. P ;; X \<triangleleft> b \<triangleright>\<^sub>r II)"
+  have 1: "Continuous (\<lambda>X. P \<Zcomp> X \<^bold>\<lhd> b \<^bold>\<rhd> II)"
     by (rel_auto)
-  have "while b do P od = (\<Sqinter>i. ((\<lambda>X. P ;; X \<triangleleft> b \<triangleright>\<^sub>r II) ^^ i) false)"
+  have "while b do P od = (\<Sqinter>i. ((\<lambda>X. P \<Zcomp> X \<^bold>\<lhd> b \<^bold>\<rhd> II) ^^ i) false)"
     by (simp add: "1" false_upred_def sup_continuous_Continuous sup_continuous_lfp while_top_def)
-  also have "... = ((\<lambda>X. P ;; X \<triangleleft> b \<triangleright>\<^sub>r II) ^^ 0) false \<sqinter> (\<Sqinter>i. ((\<lambda>X. P ;; X \<triangleleft> b \<triangleright>\<^sub>r II) ^^ (i+1)) false)"
+  also have "... = ((\<lambda>X. P \<Zcomp> X \<^bold>\<lhd> b \<^bold>\<rhd> II) ^^ 0) false \<sqinter> (\<Sqinter>i. ((\<lambda>X. P \<Zcomp> X \<^bold>\<lhd> b \<^bold>\<rhd> II) ^^ (i+1)) false)"
     by (subst Sup_power_expand, simp)
-  also have "... = (\<Sqinter>i. ((\<lambda>X. P ;; X \<triangleleft> b \<triangleright>\<^sub>r II) ^^ (i+1)) false)"
+  also have "... = (\<Sqinter>i. ((\<lambda>X. P \<Zcomp> X \<^bold>\<lhd> b \<^bold>\<rhd> II) ^^ (i+1)) false)"
     by (simp)
-  also have "... = (\<Sqinter>i. (P \<triangleleft> b \<triangleright>\<^sub>r II)\<^bold>^i ;; (false \<triangleleft> b \<triangleright>\<^sub>r II))"
+  also have "... = (\<Sqinter>i. (P \<^bold>\<lhd> b \<^bold>\<rhd> II)\<^bold>^i \<Zcomp> (false \<^bold>\<lhd> b \<^bold>\<rhd> II))"
   proof (rule SUP_cong, simp_all)
     fix i
-    show "P ;; ((\<lambda>X. P ;; X \<triangleleft> b \<triangleright>\<^sub>r II) ^^ i) false \<triangleleft> b \<triangleright>\<^sub>r II = (P \<triangleleft> b \<triangleright>\<^sub>r II) \<^bold>^ i ;; (false \<triangleleft> b \<triangleright>\<^sub>r II)"
+    show "P \<Zcomp> ((\<lambda>X. P \<Zcomp> X \<^bold>\<lhd> b \<^bold>\<rhd> II) ^^ i) false \<^bold>\<lhd> b \<^bold>\<rhd> II = (P \<^bold>\<lhd> b \<^bold>\<rhd> II) \<^bold>^ i \<Zcomp> (false \<^bold>\<lhd> b \<^bold>\<rhd> II)"
     proof (induct i)
       case 0
       then show ?case by simp
@@ -765,9 +771,9 @@ proof -
            (metis (no_types, lifting) RA1 comp_cond_left_distr cond_L6 upred_semiring.mult.left_neutral)
     qed
   qed
-  also have "... = (\<Sqinter>i\<in>{0..} \<bullet> (P \<triangleleft> b \<triangleright>\<^sub>r II)\<^bold>^i ;; [(\<not>b)]\<^sup>\<top>)"
+  also have "... = (\<Sqinter>i\<in>{0..} \<bullet> (P \<^bold>\<lhd> b \<^bold>\<rhd> II)\<^bold>^i \<Zcomp> [(\<not>b)]\<^sup>\<top>)"
     by (rel_auto)
-  also have "... = (P \<triangleleft> b \<triangleright>\<^sub>r II)\<^sup>\<star> ;; [(\<not>b)]\<^sup>\<top>"
+  also have "... = (P \<^bold>\<lhd> b \<^bold>\<rhd> II)\<^sup>\<star> \<Zcomp> [(\<not>b)]\<^sup>\<top>"
     by (metis seq_UINF_distr ustar_def)
   finally show ?thesis .
 qed
@@ -775,7 +781,7 @@ qed
 subsection \<open> Omega Algebra Laws \<close>
 
 lemma uomega_induct:
-  "P ;; P\<^sup>\<omega> \<sqsubseteq> P\<^sup>\<omega>"
+  "P \<Zcomp> P\<^sup>\<omega> \<sqsubseteq> P\<^sup>\<omega>"
   by (simp add: uomega_def, metis eq_refl gfp_unfold monoI seqr_mono)
 
 subsection \<open> Refinement Laws \<close>
@@ -796,18 +802,18 @@ lemma pre_weak_rel:
     
 lemma cond_refine_rel: 
   assumes "S \<sqsubseteq> (\<lceil>b\<rceil>\<^sub>< \<and> P)" "S \<sqsubseteq> (\<lceil>\<not>b\<rceil>\<^sub>< \<and> Q)"
-  shows "S \<sqsubseteq> P \<triangleleft> b \<triangleright>\<^sub>r Q"
+  shows "S \<sqsubseteq> P \<^bold>\<lhd> b \<^bold>\<rhd> Q"
   by (metis aext_not assms(1) assms(2) cond_def lift_rcond_def utp_pred_laws.le_sup_iff)
 
 lemma seq_refine_pred:
   assumes "(\<lceil>b\<rceil>\<^sub>< \<Rightarrow> \<lceil>s\<rceil>\<^sub>>) \<sqsubseteq> P" and "(\<lceil>s\<rceil>\<^sub>< \<Rightarrow> \<lceil>c\<rceil>\<^sub>>) \<sqsubseteq> Q"
-  shows "(\<lceil>b\<rceil>\<^sub>< \<Rightarrow> \<lceil>c\<rceil>\<^sub>>) \<sqsubseteq> (P ;; Q)"
+  shows "(\<lceil>b\<rceil>\<^sub>< \<Rightarrow> \<lceil>c\<rceil>\<^sub>>) \<sqsubseteq> (P \<Zcomp> Q)"
   using assms by rel_auto
     
 lemma seq_refine_unrest:
   assumes "out\<alpha> \<sharp> b" "in\<alpha> \<sharp> c"
   assumes "(b \<Rightarrow> \<lceil>s\<rceil>\<^sub>>) \<sqsubseteq> P" and "(\<lceil>s\<rceil>\<^sub>< \<Rightarrow> c) \<sqsubseteq> Q"
-  shows "(b \<Rightarrow> c) \<sqsubseteq> (P ;; Q)"
+  shows "(b \<Rightarrow> c) \<sqsubseteq> (P \<Zcomp> Q)"
   using assms by rel_blast 
     
 subsection \<open> Preain and Postge Laws \<close>
@@ -839,7 +845,7 @@ lemma Pre_assume [prepost]:
   by (rel_auto)
     
 lemma Pre_seq:
-  "Pre(P ;; Q) = Pre(P ;; [Pre(Q)]\<^sup>\<top>)"
+  "Pre(P \<Zcomp> Q) = Pre(P \<Zcomp> [Pre(Q)]\<^sup>\<top>)"
   by (rel_auto)
     
 lemma Pre_disj [prepost]:
@@ -857,7 +863,7 @@ lemma Pre_conj_indep [prepost]: "\<lbrakk> {$a,$a\<acute>} \<natural> P; $a\<acu
   by (rel_auto, metis lens_override_def lens_override_idem)
 
 lemma assume_Pre [prepost]:
-  "[Pre(P)]\<^sup>\<top> ;; P = P"
+  "[Pre(P)]\<^sup>\<top> \<Zcomp> P = P"
   by (rel_auto)
 
 end
