utp_wlp.thy
@@ -7,7 +7,7 @@ begin
 named_theorems wp
 
 definition wlp_pred :: "('s\<^sub>1 \<leftrightarrow> 's\<^sub>2) \<Rightarrow> ('s\<^sub>2 \<Rightarrow> bool) \<Rightarrow> ('s\<^sub>1 \<Rightarrow> bool)" where
-[rel]: "wlp_pred Q r = pre (\<not> (Q ;; ((\<not> r\<^sup><)\<^sub>u)) :: ('s\<^sub>1 \<leftrightarrow> 's\<^sub>2))"
+[rel]: "wlp_pred Q r = pre (\<not> (Q \<Zcomp> ((\<not> r\<^sup><)\<^sub>u)) :: ('s\<^sub>1 \<leftrightarrow> 's\<^sub>2))"
 
 expr_ctr wlp_pred
 
@@ -17,7 +17,7 @@ syntax
 translations
   "_wlp Q r" == "CONST wlp_pred Q (r)\<^sub>e"
 
-lemma wlp_seq [wp]: "(P ;; Q) wlp b = P wlp (Q wlp b)"
+lemma wlp_seq [wp]: "(P \<Zcomp> Q) wlp b = P wlp (Q wlp b)"
   by (rel_auto)
 
 lemma wlp_assigns [wp]: "\<langle>\<sigma>\<rangle>\<^sub>a wlp b = (\<sigma> \<dagger> b)\<^sub>e"
